src/Bedrock/Field/Interface/Compilation2.v
@@ -12,7 +12,7 @@ Section Compile.
   Context {locals_ok : map.ok locals}.
   Context {ext_spec_ok : Semantics.ext_spec.ok ext_spec}.
   Context {field_parameters : FieldParameters}
-          {field_representaton : FieldRepresentation}
+          {field_representation : FieldRepresentation}
           {field_representation_ok : FieldRepresentation_ok}.
 
   Definition maybe_bounded mbounds v :=
@@ -47,25 +47,36 @@ Section Compile.
     sepsimpl; simpl in *; eauto using relax_bounds.
   Qed.
 
-  Lemma FElem'_from_bytes
+  Lemma FElem'_iff_bytes
     : forall px : word.rep,
-      Lift1Prop.iff1 (Placeholder px) (Lift1Prop.ex1 (FElem None px)).
-  Proof using mem_ok word_ok.
+      Lift1Prop.iff1 (Lift1Prop.ex1 (Placeholder px)) (Lift1Prop.ex1 (FElem None px)).
+  Proof using field_representation_ok mem_ok word_ok.
     unfold FElem.
     intros.
     split; intros.
     {
-      apply FElem_from_bytes in H.
-      destruct H.
+      destruct H as [bs H].
+      apply Placeholder_impl_FElem_bytes in H.
       do 2 eexists.
       sepsimpl; simpl; eauto.
     }
     {
-      destruct H as [? [? ?]].
+      destruct H as [ws [? H]].
       sepsimpl.
-
-      eapply FElem_to_bytes; eauto.
+      eexists.
+      eapply Placeholder_impl_FElem_words; eauto.
     }
+  Qed.
+
+  Lemma FElem'_to_bytes
+    : forall bounds px x,
+      Lift1Prop.impl1 (FElem bounds px x) (Lift1Prop.ex1 (Placeholder px)).
+  Proof.
+    intros. cbv [FElem]. intros m [f F].
+    extract_ex1_and_emp_in F.
+    sepsimpl.
+    eexists. eapply Placeholder_impl_FElem_words.
+    eassumption.
   Qed.
 
   #[refine]
@@ -77,14 +88,20 @@ Section Compile.
   Proof.
     {
       intros; intros m H.
-      apply FElem'_from_bytes.
+      apply FElem'_to_bytes in H.
+      cbv[Placeholder] in *.
+      sepsimpl. 
       eexists.
-      eapply drop_bounds_FElem; eauto.
+      pose felem_size_ok.
+      ssplit; try eassumption.
+      lia.
     }
     {
       intros; intros m H.
-      apply FElem'_from_bytes.
-      eauto.
+      apply FElem'_iff_bytes.
+      cbv [Memory.anybytes Placeholder] in *. sepsimpl.
+      eexists; try eassumption.
+      sepsimpl; try eassumption.
     }
   Defined.
 
@@ -97,21 +114,19 @@ Section Compile.
     end; eauto;
     sepsimpl; repeat straightline'; subst; eauto.
 
-
   Local Hint Extern 1 (spec_of _) => (simple refine (@spec_of_BinOp _ _ _ _ _ _ _ _ _ _)) : typeclass_instances.
   Local Hint Extern 1 (spec_of _) => (simple refine (@spec_of_UnOp _ _ _ _ _ _ _ _ _ _)) : typeclass_instances.
 
   Lemma compile_binop {name} {op: BinOp name}
-        {tr m l functions} x y:
+        {tr m l functions} x y out:
     let v := bin_model x y in
     forall P (pred: P v -> predicate) (k: nlet_eq_k P v) k_impl
-           Rx Ry Rout out x_ptr x_var y_ptr y_var out_ptr out_var
-           bound_out,
+           Rx Ry Rout x_ptr x_var y_ptr y_var out_ptr out_var,
 
       (_: spec_of name) functions ->
 
       map.get l out_var = Some out_ptr ->
-      (FElem bound_out out_ptr out * Rout)%sep m ->
+      (Placeholder out_ptr out * Rout)%sep m ->
 
       (FElem (Some bin_xbounds) x_ptr x * Rx)%sep m ->
       (FElem (Some bin_ybounds) y_ptr y * Ry)%sep m ->
@@ -135,7 +150,7 @@ Section Compile.
         (cmd.call [] name [expr.var out_var; expr.var x_var; expr.var y_var])
         k_impl
       <{ pred (nlet_eq [out_var] v k) }>.
-  Proof using ext_spec_ok locals_ok mem_ok word_ok.
+  Proof using ext_spec_ok locals_ok mem_ok word_ok field_representation_ok.
     repeat straightline'.
     unfold FElem in *.
     sepsimpl.
@@ -150,15 +165,15 @@ Section Compile.
       eauto.
   Qed.
 
-  Lemma compile_unop {name} (op: UnOp name) {tr m l functions} x:
+  Lemma compile_unop {name} (op: UnOp name) {tr m l functions} x out:
     let v := un_model x in
     forall P (pred: P v -> predicate) (k: nlet_eq_k P v) k_impl
-           Rin Rout out x_ptr x_var out_ptr out_var out_bounds,
+           Rin Rout x_ptr x_var out_ptr out_var,
 
       (_: spec_of name) functions ->
 
       map.get l out_var = Some out_ptr ->
-      (FElem out_bounds out_ptr out * Rout)%sep m ->
+      (Placeholder out_ptr out * Rout)%sep m ->
 
       (FElem (Some un_xbounds) x_ptr x * Rin)%sep m ->
       map.get l x_var = Some x_ptr ->
@@ -231,16 +246,16 @@ Section Compile.
 
   Local Hint Extern 1 (spec_of _) => (simple refine (@spec_of_felem_copy _ _ _ _ _ _ _ _)) : typeclass_instances.
 
-  Lemma compile_felem_copy {tr m l functions} x :
+  Lemma compile_felem_copy {tr m l functions} x out :
     let v := x in
     forall P (pred: P v -> predicate) (k: nlet_eq_k P v) k_impl
-           R x_ptr x_var out out_ptr out_var x_bound out_bound,
+           R x_ptr x_var out_ptr out_var x_bound,
 
       spec_of_felem_copy functions ->
 
       map.get l out_var = Some out_ptr ->
 
-      (FElem x_bound x_ptr x * FElem out_bound out_ptr out * R)%sep m ->
+      (FElem x_bound x_ptr x * Placeholder out_ptr out * R)%sep m ->
       map.get l x_var = Some x_ptr ->
 
       (let v := v in
@@ -272,15 +287,15 @@ Section Compile.
 
   Local Hint Extern 1 (spec_of _) => (simple refine (@spec_of_from_word _ _ _ _ _ _ _ _)) : typeclass_instances.
 
-  Lemma compile_from_word {tr m l functions} x:
+  Lemma compile_from_word {tr m l functions} x out:
     let v := F.of_Z _ x in
     forall P (pred: P v -> predicate) (k: nlet_eq_k P v) k_impl
-           R (wx : word) out out_ptr out_var out_bounds,
+           R (wx : word) out_ptr out_var,
 
       spec_of_from_word functions ->
 
       map.get l out_var = Some out_ptr ->
-      (FElem out_bounds out_ptr out * R)%sep m ->
+      (Placeholder out_ptr out * R)%sep m ->
 
       word.unsigned wx = x ->
 
@@ -430,6 +445,7 @@ is_var v; simple eapply compile_felem_copy; shelve : compiler.
 
 #[export] Hint Immediate relax_bounds_FElem : ecancel_impl.
 #[export] Hint Immediate drop_bounds_FElem : ecancel_impl.
+#[export] Hint Extern 1 (Lift1Prop.impl1 (FElem _ ?x _) (Placeholder ?x)) =>(eapply FElem'_to_bytes) : ecancel_impl.
 
 
 #[export] Hint Extern 1 (spec_of _) => (simple refine (@spec_of_BinOp _ _ _ _ _ _ _ _ _ _)) : typeclass_instances.
