src/Bedrock/Field/Interface/Representation.v
@@ -34,7 +34,6 @@ Section Representation.
             and for word-by-word Montgomery, the argument must be pulled out of the Montgomery domain*)
           (eval_transformation : list Z -> list Z).
 
-
   Definition eval_words : list word -> F M_pos :=
     fun ws =>
       F.of_Z _ (Positional.eval weight n (eval_transformation (map word.unsigned ws))).
@@ -58,6 +57,11 @@ Section Representation.
       tight_bounds := tight_bounds;
     }.
 
+  Context (felem_size_ok : felem_size_in_bytes <= 2 ^ width).
+
   Local Instance frep_ok : FieldRepresentation_ok.
-  Proof. split. cbn [bounded_by frep]; intros. apply relax_bounds; auto. Qed.
+  Proof.
+    split. cbn [bounded_by frep]; intros. apply relax_bounds; auto. 
+    apply felem_size_ok.
+  Qed.
 End Representation.
